quase pronto

Conjunto.dfy
@@ -1,44 +1,217 @@
-class {:autocontracts} Conjunto{
-    //implementacao
-    var arr: array<int>;
-    //tamanho do conjunto, pode ser usado como o atributo cauda da Fila
+function toset(s: seq<int>): set<int>
+{
+    set x | x in s
+}
+
+function method tosetMethod(arr: array<int>): set<int>
+reads arr
+{
+    var s := arr[..];
+    set x | x in s
+}
+
+class {:autocontracts} ConjuntoInt {
+    //Implementação
+    var a: array<int>;
     var tamanho: nat;
-    //abstracao
-    ghost var Conteudo: set<int> ;
+    //Abstração
+    ghost var conteudo: seq<int>;
 
-    predicate Valid(){
-        arr.Length > 0 &&
-        tamanho <= arr.Length &&
-        (forall i, j :: 0 <= i < tamanho && 0 <= j < tamanho && i != j ==> arr[i] != arr[j]) &&
-        (forall num: int :: num in Conteudo <==> exists i: nat :: i < tamanho && arr[i] == num)
-
+    //invariante de classe
+    predicate Valid()
+    {
+        a.Length > 0
+        && 0 <= tamanho <= a.Length
+        && |conteudo| == tamanho
+        && conteudo == a[..tamanho]
+        && (forall i, j :: 0 <= i < j < tamanho ==> a[i] != a[j])
     }
+
     constructor()
-    ensures Conteudo == {};
+    ensures conteudo == []
     {
-        arr := new int[20];
+        a := new int[5];
         tamanho := 0;
-        Conteudo := {};
+        conteudo := [];
     }
 
-    //to do: abaixo
-    method add(num: int) returns (b : bool)
-    ensures Conteudo == (old(Conteudo) + {num});
+    method pertence(e:int) returns (r:bool)
+    ensures r <==> e in toset(conteudo)
+    ensures toset(conteudo) == toset(old(conteudo))
+    ensures |conteudo| == old(|conteudo|)
+    ensures conteudo == old(conteudo)
     {
-
+        var i := 0;
+        while i < tamanho
+        invariant 0 <= i <= tamanho
+        invariant forall j :: 0 <= j < i ==> a[j] != e
+        {
+            if a[i] == e
+            {
+                return true;
+            }
+            i := i + 1;
+        }
+        return false;
     }
 
-    method remove() returns (b: bool)
+    method adicionar(e:int) returns (r:bool)
+    ensures r <==> e !in toset(old(conteudo))
+    ensures r ==> toset(conteudo) == toset(old(conteudo)) + {e}
+    ensures !r ==> toset(conteudo) == toset(old(conteudo))
+    {
+        var p := pertence(e);
+        if p
+        {
+            r := false;
+        }
+        else
+        {
+            if tamanho == a.Length
+            {
+                var b := new int[2 * tamanho];
+                forall i | 0 <= i < tamanho
+                {
+                    b[i] := a[i];
+                }
+                a := b;
+            }
+            a[tamanho] := e;
+            tamanho := tamanho + 1;
+            conteudo := conteudo + [e];
+            r := true;
+        }
+    }
 
-    method contains(i: int) returns (b: bool)
+    method buscaNoArray(e: int) returns (pos: int)
+    ensures conteudo == old(conteudo)
+    ensures |conteudo| == |old(conteudo)|
+    ensures (e !in toset(conteudo)) <==> pos == -1    
+    ensures (e in toset(conteudo)) <==> 0 <= pos < tamanho && conteudo[pos] == e
+    ensures -1 <= pos < tamanho
+    {
+        pos := -1;
+        var i:nat := 0;
+        
+        while i < tamanho
+        invariant 0 <= i <= tamanho
+        invariant forall j :: 0 <= j < i ==> a[j] != e
+        {
+            if (a[i] == e) {
+                return i;
+            }
+            i := i + 1;
+        }
+    }
+
+    method remover(e:int) returns (r:bool)
+    ensures r <==> e in toset(old(conteudo))
+    ensures r  ==> toset(conteudo) == toset(old(conteudo)) - {e} && |conteudo| == |old(conteudo)| - 1
+    ensures !r ==> toset(conteudo) == toset(old(conteudo)) && |conteudo| == |old(conteudo)|
+    {
+        var p := pertence(e);
+        if !p
+        {
+            r := false;
+        }
+        else
+        {
+            assert e in conteudo;
+            var pos := buscaNoArray(e);
+            assert 0 <= pos < tamanho;
+            assert |conteudo| == tamanho;
+            tamanho := tamanho-1;
+            a[pos] := a[tamanho];
+            conteudo := a[..tamanho];
+            assert pos < old(|conteudo|);
+            assert conteudo[..pos] == old(conteudo)[..pos];
+            assert conteudo[pos] == old(conteudo)[|old(conteudo)|-1];
+            if pos < old(tamanho)-1{
+                assert 0 <= pos < |old(conteudo)|;
+                assert |old(conteudo)| == old(tamanho);
+                assert conteudo[..pos] == old(conteudo)[..pos];
+                //assert conteudo == old(conteudo)[..pos] + [old(conteudo)[old(tamanho)-1]] + old(conteudo)[pos+1..];
+            }
+            else if pos == old(tamanho)-1{
+                assert pos == |old(conteudo)|-1;
+                //assert conteudo == old(conteudo)[..pos] + [old(conteudo)[old(tamanho)-1]];
+            }
+            r := true;
+        }
+    }
 
     method getSize() returns (s: int)
+    ensures s == |conteudo|
+    ensures conteudo == old(conteudo)
+    {
+        return tamanho;
+    }
 
     method isEmpty() returns (b: bool)
+    ensures b <==> (|conteudo| == 0)
+    ensures conteudo == old(conteudo)
+    {
+        return (tamanho==0);
+    }
 
-    method union(set2: Conjunto) returns (c: Conjunto)
+    method union(set2: ConjuntoInt) returns (c: ConjuntoInt)
+    ensures conteudo == old(conteudo)
+    ensures set2.conteudo == old(set2.conteudo)
+    ensures toset(c.conteudo) == toset(conteudo) + toset(set2.conteudo)
+    ensures forall e :: (e in conteudo) || (e in set2.conteudo) <==> (e in c.conteudo)
+    //{
+    //    c := new ConjuntoInt();
+    //    var conj1 := (set x | x in tosetMethod(a));
+    //    var conj2 := (set x | x in tosetMethod(set2.a));
+    //    var conjResp := conj1 + conj2;
+    //    while conjResp != {}
+    //    decreases |conjResp|
+    //    {
+    //      var i: int :| i in conjResp;
+    //      conjResp := conjResp - {i};
+    //      c.adicionar(i);
+    //    }
+    //}
 
-    method intersec(set2: Conjunto) returns (c: Conjunto)
+    method intersec(set2: ConjuntoInt) returns (c: ConjuntoInt)
+    ensures conteudo == old(conteudo)
+    ensures set2.conteudo == old(set2.conteudo)
+    ensures toset(c.conteudo) == toset(conteudo) * toset(set2.conteudo)
+    ensures forall e :: (e in conteudo) && (e in set2.conteudo) <==> (e in c.conteudo)
+    //{
+    //    c := new ConjuntoInt();
+    //    var conj1 := (set x | x in tosetMethod(a));
+    //    var conj2 := (set x | x in tosetMethod(set2.a));
+    //    var conjResp := conj1 * conj2;
+    //    while conjResp != {}
+    //    decreases |conjResp|
+    //    {
+    //      var i: int :| i in conjResp;
+    //      conjResp := conjResp - {i};
+    //      c.adicionar(i);
+    //    }
+    //}
 
-    method minus(sec2: Conjunto) returns (c: Conjunto)
+    method minus(set2: ConjuntoInt) returns (c: ConjuntoInt)
+    ensures conteudo == old(conteudo)
+    ensures set2.conteudo == old(set2.conteudo)
+    ensures toset(c.conteudo) == toset(conteudo) - toset(set2.conteudo)
+    ensures forall e :: (e in conteudo) && (e !in set2.conteudo) <==> (e in c.conteudo)
+    //{
+    //    c := new ConjuntoInt();
+    //    var conj1 := (set x | x in tosetMethod(a));
+    //    var conj2 := (set x | x in tosetMethod(set2.a));
+    //    var conjResp := conj1 - conj2;
+    //    while conjResp != {}
+    //    decreases |conjResp|
+    //    {
+    //      var i: int :| i in conjResp;
+    //      conjResp := conjResp - {i};
+    //      c.adicionar(i);
+    //    }
+    //}
+}
+
+method Main(){
+    var conj := new ConjuntoInt();
 }
